AVM/Program.lean
@@ -3,6 +3,7 @@ import AVM.Class.Label
 import Init.Data.Fin.Lemmas
 import AVM.Object
 import AVM.Class
+import AVM.Ecosystem
 
 namespace AVM
 
@@ -11,6 +12,8 @@ open Class
 inductive PType : Type (u + 1) where
   | Object : Class.Label → PType
   | Reference : Class.Label → PType
+  | SomeType : SomeType → PType
+  | Program : (args : List PType) → (ret : PType) →  PType
 
 def LocalVars (n : Nat) : Type (u + 1) := Vector PType n
 
@@ -19,51 +22,104 @@ namespace LocalVars
 def extend (v : PType) (l : LocalVars n) : LocalVars (n + 1) :=
     l.push v
 
-infixr:67 " :: " => extend
+infixr:67 " ▹ " => extend
 
 end LocalVars
 
 structure LocalVar {n : Nat} (Γ : LocalVars n) (ty : PType) : Type where
   ix : Fin n
-  typed : Γ.get ix = ty
+  typed : Γ.get ix = ty := by rfl
 
-inductive Expr {n : Nat} (Γ : LocalVars n) : PType → Type (u + 1) where
+inductive Expr (Γ : LocalVars n) : PType → Type (u + 1) where
   | constRef {lab : Class.Label} (ref : Reference lab) : Expr Γ (.Reference lab)
   | var {ty : PType} (v : LocalVar Γ ty) : Expr Γ ty
+  | const {t : SomeType} : t.type → Expr Γ (.SomeType t)
 
-inductive Program : {n : Nat} → LocalVars n → Type (u + 1) where
-  | constructorCall
-      {Γ : LocalVars n}
-      {clab : Class.Label.{u}}
-      {constructorId : clab.ConstructorId}
-      (constr : Constructor constructorId)
-      (args : constructorId.Args.type)
-      (prog : Program (.Reference clab :: Γ))
-      : Program Γ
-  | destructorCall
-      {Γ : LocalVars n}
-      {clab : Class.Label.{u}}
-      {destructorId : clab.DestructorId}
-      (destr : Destructor destructorId)
-      (args : destructorId.Args.type)
-      (self : Expr Γ (.Reference clab))
-      (prog : Program Γ)
-      : Program Γ
-  | methodCall
+inductive Exprs (Γ : LocalVars n) : (len : Nat) → Type (u + 1) where
+  | nil : Exprs Γ 0
+  | cons (ty : PType) {len : Nat} (e : Expr Γ ty) (es : Exprs Γ len) : Exprs Γ (len + 1)
+
+def Exprs.typeList {Γ : LocalVars n} (es : Exprs Γ l) : List PType := match es with
+  | .nil => []
+  | .cons ty _e es => ty :: es.typeList
+
+def typeOfExt : PType.{u} → Type u := fun
+  | .Object l => Object l
+  | .Program args ret => args.map typeOfExt |>.Product → typeOfExt ret
+  | .Reference l => ULift (Reference l)
+  | .SomeType l => l.type
+
+def typesOf {Γ : LocalVars n} : Exprs Γ l → LocalVars l := fun
+  | .nil => Vector.ofFn fun x => nomatch x
+  | .cons ty _e es => typesOf es |>.push ty
+
+def typesOfExt.{u} (tys : List PType) : Type u := tys.map typeOfExt |>.Product
+
+infixr:67 " ::: " => Exprs.cons
+
+instance LocalVars.instMembership {n : Nat} : Membership PType (LocalVars n) := Vector.instMembership
+
+inductive Program.{u} : {n : Nat} → LocalVars.{u} n → (ret : PType) → Type (u + 1) where
+  -- FIXME I haven't still figured out a way to formalize constructor calls.
+  -- The sort reification that I've done here should be replaced.
+  -- But then, how does one specify the object that's built in a constructor?
+  -- It's tempting to use Lean4 records, but then how do we pass arguments that are created during program execution?
+  -- I think the solution is to add Object expressions to Expr. But this seems complicated
+  -- There is probably a better way
+  | callConstructor
+     {Γ : LocalVars.{u} n}
+     {ret : PType}
+     {clab : Class.Label}
+     {nargs : Nat}
+     (args : Exprs Γ nargs)
+     (fn : typesOfExt args.typeList → Object clab)
+     (prog : Program (.Reference clab ▹ Γ) ret)
+     : Program Γ ret
+  | let
      {Γ : LocalVars n}
+     {ret : PType}
+     {exprTy : PType}
+     (expr : Expr Γ exprTy)
+     (prog : Program (exprTy ▹ Γ) ret)
+     : Program Γ ret
+  | call
+     {Γ : LocalVars n}
+     {ret : PType}
+     {ret' : PType}
+     {nargs : Nat}
+     (args : Exprs Γ nargs)
+     (fn : Expr Γ (.Program (typesOf args).toList ret'))
+     (prog : Program (ret' ▹ Γ) ret)
+     : Program Γ ret
+  | pure
+     {Γ : LocalVars n}
+     {ret : PType}
+     (e : Expr Γ ret)
+     : Program Γ ret
+  | store
+     {Γ : LocalVars n}
+     {ret : PType}
      {clab : Class.Label.{u}}
-     {methodId : clab.MethodId}
-     (method : Method methodId)
-     (args : methodId.Args.type)
-     (self : Expr Γ (.Reference clab))
-     (prog : Program Γ)
-     : Program Γ
+     (ref : Expr Γ (.Reference clab))
+     (obj : Object clab)
+     (prog : Program Γ ret)
+     : Program Γ ret
+  | allocate
+     {Γ : LocalVars n}
+     {ret : PType}
+     (clab : Class.Label.{u})
+     (prog : Program (.Reference clab ▹ Γ) ret)
+     : Program Γ ret
   | deref
      {Γ : LocalVars n}
+     {ret : PType}
      {clab : Class.Label.{u}}
      (ref : Reference clab)
-     (prog : Program (.Object clab :: Γ))
-     : Program Γ
+     (prog : Program (.Object clab ▹ Γ) ret)
+     : Program Γ ret
 
-def TopProgram : Type (u + 1) :=
-    Program (Vector.emptyWithCapacity 0)
+def TopProgram (ret : PType) : Type (u + 1) :=
+    Program (Vector.emptyWithCapacity 0) ret
+
+def Program.noop {Γ : LocalVars n} : Program Γ (.SomeType ⟨Unit⟩) :=
+  Program.pure (.const .unit)
